

5651 HW 1 - Matthew Pipes

$$1(a) \sum_{k=1}^{\infty} \frac{1}{2^k} = 1$$

Utilizing the sum of an infinite geometric series formula $S = \frac{a_1}{1-r}$

with $a_1 = \frac{1}{2}$, $r = \frac{1}{2}$ yields $S = \frac{\frac{1}{2}}{\frac{1}{2}} = 1$, as desired.

$$1(b) \sum_{k=1}^{\infty} q^{k-1} p = 1$$

Begin by re-writing q^{k-1} as $\frac{q^k}{q}$, and moving terms without k out of the summation $\rightarrow \frac{p}{q} \sum_{k=1}^{\infty} q^k$

Expand the first few terms to seek a pattern

$$\rightarrow \frac{p}{q} (q + q^2 + q^3 + \dots) \rightarrow p(1 + q + q^2 + \dots)$$

Note this is a geometric series with $a_1 = p$ and $r = q = 1-p$.

So using the infinite geometric series formula once more yields

$$\frac{p}{1-(1-p)} = \frac{p}{p} = 1. \quad \text{Thus we have shown}$$

$$\sum_{k=1}^{\infty} q^{k-1} p = 1.$$

2. Show that

$$\sum_{k=0}^{\infty} \frac{e^{-\lambda} \lambda^k}{k!} = 1. \quad \text{Move } e^{-\lambda} \text{ out of summation.}$$

$$\rightarrow e^{-\lambda} \cdot \sum_{k=0}^{\infty} \frac{\lambda^k}{k!} \quad \text{Note, the Taylor series expansion for}$$
$$e^x = \sum_{n=0}^{\infty} \frac{x^n}{n!}.$$

$$\text{Thus, } \sum_{k=0}^{\infty} \frac{\lambda^k}{k!} = e^{\lambda}. \quad \text{Finally,}$$

$$e^{-\lambda} \cdot e^{\lambda} = e^0 = 1, \text{ as desired.}$$

③ If $X \sim \text{Geo}(p)$, find $E(X)$ in as many ways possible.

$$E(X) = \sum_{x=1}^{\infty} x P(X=x). \quad P(X=x) = p(1-p)^{x-1} \quad \text{Thus,}$$

$$E(X) = \sum_{x=1}^{\infty} x p (1-p)^{x-1}.$$

List some of the first elements:

$$p + 2p(1-p) + 3p(1-p)^2 + 4p(1-p)^3 + \dots \quad \text{Since } q = 1-p$$

$$E(X) = p + 2qp + 3q^2p + 4q^3p + \dots \quad (1)$$

Multiply by q , form new equation

$$qE(X) = qp + 2q^2p + 3q^3p + \dots \quad (2)$$

$$\text{Perform } (1) - (2): \quad E(X) - qE(X) = p + qp + q^2p + q^3p + \dots$$

Factor $E(X)$ on LHS. Factor p on RHS. RHS becomes infinite geometric series with $\text{sum} = 1$.

$$E(X) \underbrace{[1-q]}_p = 1$$

$$pE(X) = 1, \quad \text{thus } E(X) = \frac{1}{p}$$

Problem 4: If $X \sim \text{Poi}(\lambda)$, find $E(X)$

$$E(X) = \sum_{x=0}^{\infty} x \cdot \frac{e^{-\lambda} \lambda^x}{x!}$$

Proceed by factoring the constant term $e^{-\lambda}$ out. and see that the first term is zero, so we can begin at $x=1$.

$$= e^{-\lambda} \sum_{x=1}^{\infty} \frac{x \cdot \lambda^x}{x!}$$

Can clear x in numerator by rewriting $x!$ as $x(x-1)!$

$$= e^{-\lambda} \sum_{x=1}^{\infty} \frac{\lambda^x}{(x-1)!}$$

Strip off a λ term, rewrite λ^x as $\lambda^{x-1} \cdot \lambda$

$$= e^{-\lambda} \sum_{x=1}^{\infty} \frac{\lambda^{x-1} \cdot \lambda}{(x-1)!}$$

Move constant λ term out. Let $l = x-1$

$$= \lambda \cdot e^{-\lambda} \cdot \sum_{x=1}^{\infty} \frac{\lambda^{x-1}}{(x-1)!}$$

Notice that this is the Taylor series expansion for e^{λ} , like earlier. Thus,

$$E(X) = \lambda \cdot e^{-\lambda} \cdot e^{\lambda} = \lambda e^0 = \lambda.$$

Math 5651 - Matthew Piers - HW 1

Problem 5: Prove $E(X) + E(Y) = E(X+Y)$

Given $E(X+Y) = \sum_i \sum_j (x_i + y_j) \cdot P(X=x_i, Y=y_j)$

We Distribute $(x_i + y_j)$ with $P(X=x_i, Y=y_j)$:

$$\sum_i \sum_j x_i \cdot P(X=x_i, Y=y_j) + y_j \cdot P(X=x_i, Y=y_j)$$

We Split the summations:

$$\sum_i \sum_j x_i \cdot P(X=x_i, Y=y_j) + \sum_i \sum_j y_j \cdot P(X=x_i, Y=y_j)$$

x_i does not depend on j , move out by one summation.

Flip $\sum_i \sum_j$ in the double summation with y_j . Move y_j out one summation.

$$\sum_i x_i \underbrace{\sum_j P(X=x_i, Y=y_j)}_{P(X=x_i)} + \sum_j y_j \underbrace{\sum_i P(X=x_i, Y=y_j)}_{P(Y=y_j)}, \text{ thus}$$

$$\sum_i x_i \cdot P(X=x_i) + \sum_j y_j \cdot P(Y=y_j). \text{ By definition of Expected Value:}$$

$$E(X) + E(Y). \text{ Thus, } E(X+Y) = E(X) + E(Y).$$

□

	$Y=1$	$Y=2$	$Y=3$	$Y=4$	$Y=5$	$Y=6$
$P(X=1 Y=1)$		$X=2$ $\frac{1}{4} \cdot \frac{1}{2}$	$X=3$ $\frac{1}{8} \cdot \frac{1}{2}$	$X=4$ $\frac{1}{16} \cdot \frac{1}{2}$	$X=5$ $\frac{1}{32} \cdot \frac{1}{2}$	$X=6$ $\frac{1}{64} \cdot \frac{1}{2}$
$X=1$ $\frac{1}{2} \cdot \frac{1}{2}$		$X=1$	$X=2$ $\frac{3}{8} \cdot \frac{1}{2}$	$X=3$ $\frac{4}{16} \cdot \frac{1}{2}$	$X=4$ $\frac{5}{32} \cdot \frac{1}{2}$	$X=5$ $\frac{6}{64} \cdot \frac{1}{2}$
$P(X=0 Y=1)$ and so on		$X=0$ $\frac{1}{2} \cdot \frac{1}{2}$	$X=1$	$X=2$ $\frac{6}{16} \cdot \frac{1}{2}$	$X=3$ $\frac{10}{32} \cdot \frac{1}{2}$	$X=4$ $\frac{20}{64} \cdot \frac{1}{2}$
$X=0$ $\frac{1}{2} \cdot \frac{1}{2}$		$X=0$	$X=0$ $\frac{3}{8} \cdot \frac{1}{2}$	$X=1$ $\frac{6}{16} \cdot \frac{1}{2}$	$X=2$ $\frac{10}{32} \cdot \frac{1}{2}$	$X=3$ one too $\frac{13}{64} \cdot \frac{1}{2}$ any squares in this column
						$X=2$ $\frac{6}{64} \cdot \frac{1}{2}$
						$X=1$ $\frac{1}{64} \cdot \frac{1}{2}$
						$X=0$

Thus, from the previous drawing, we can begin to build a solution.

We note that Y follows a uniform distribution, thus $P(Y=y) = \frac{1}{6}$ in all cases.

$P(X=x|Y=y)$ yields the height of a segment within the specific column

$P(X=x|Y=y) \cdot P(Y=y)$ yields the area of the prior segment from the whole solution space.

And, using the law of total probability, we can calculate that

$$P(X=x) \text{ using } \sum_{y=1}^6 P(X=x|Y=y) \cdot P(Y=y)$$

Since X describes a binomial distribution, and Y describes a uniform distribution, we have,

$$P(X=x) = \sum_{y=\max(1,x)}^6 \binom{y}{x} \left(\frac{1}{2}\right)^x \left(\frac{1}{2}\right)^{y-x} \cdot \frac{1}{6}$$

or more cleanly

$$P(X=x) = \frac{1}{6} \sum_{y=\max(1,x)}^6 \binom{y}{x} \left(\frac{1}{2}\right)^y$$